add test

Test/git-issues/git-issue-2500.dfy
@@ -28,18 +28,36 @@ class Cl extends M.Tr {
   { false }
 }
 
-trait Trait {
-  predicate Even(i: nat)
-    //ensures if i == 0 then true else (i % 2 == 0) == Odd(i-1)
-  predicate Odd(i: nat)
-    ensures if i == 0 then true else (i % 2 == 1) == Even(i-1)
+module SSCinClass {
+  trait Trait {
+    predicate Even(i: nat)
+    predicate Odd(i: nat)
+      ensures if i == 0 then true else (i % 2 == 1) == Even(i-1)
+  }
+
+  class Class extends Trait {
+    predicate Even(i: nat)
+  { if i == 0 then true else Odd(i-1) }
+    predicate Odd(i: nat)
+      ensures if i == 0 then true else (i % 2 == 1) == Even(i-1)
+    { if i == 0 then false else Even(i-1) }
+  }
 }
 
-class Class extends Trait {
-  predicate Even(i: nat)
-    //ensures if i == 0 then true else (i % 2 == 0) == Odd(i-1)
- { if i == 0 then true else Odd(i-1) }
-  predicate Odd(i: nat)
-    ensures if i == 0 then true else (i % 2 == 1) == Even(i-1)
-  { if i == 0 then false else Even(i-1) }
+module SSCinBoth {
+  trait Trait {
+    predicate Even(i: nat)
+      ensures if i == 0 then true else (i % 2 == 0) == Odd(i-1)
+    predicate Odd(i: nat)
+      ensures if i == 0 then true else (i % 2 == 1) == Even(i-1)
+  }
+
+  class Class extends Trait {
+    predicate Even(i: nat)
+      ensures if i == 0 then true else (i % 2 == 0) == Odd(i-1)
+  { if i == 0 then true else Odd(i-1) }
+    predicate Odd(i: nat)
+      ensures if i == 0 then true else (i % 2 == 1) == Even(i-1)
+    { if i == 0 then false else Even(i-1) }
+  }
 }
